jsonstar/JsonStar.Schema.Ast.Types.fst
@@ -1,0 +1,128 @@
+/// This module provides a simplified view of F* terms we want to translate into json-schema
+module JsonStar.Schema.Ast.Types
+
+// ..\packages\FStar.Windows.Ocaml.Unofficial.0.4.0\tools\bin\fstar.exe  --error_contexts true --odir obj\Debug\extracted --codegen FSharp --use_hints --record_hints JsonStar.Schema.Ast.Types.fst --extract "+JsonStar.Schema.Ast.Types"
+
+let description (desc : string) : Tot unit = ()
+let defaultValue (v : string) : Tot unit = ()
+let readOnly : unit = ()
+/// Provided value has to be known at compile-time
+let readOnlyIf (v : bool) : Tot unit = ()
+
+type format_type = 
+    | Percentage
+    | Date
+
+let format_type_to_string (x : format_type) = 
+    match x with
+    | Percentage -> "percentage"
+    | Date       -> "date"
+
+let format (f : format_type) : Tot unit = ()
+
+/// Attributes that can be associated with anything that represents a field in json-schema
+type value_attributes = 
+    {
+        _description  : option string;
+        _defaultValue : option string;
+        _readOnly     : option bool;
+        _format       : option format_type;
+    }
+
+/// Attributes that can be associated with anything that represents an object in json-schema
+type object_attributes =
+    {
+        _description : option string;
+        // Id, schemaVersion, title, AllowAdditionalProperties ... (?)
+    }
+
+type number_refinement = 
+    | Minimum : v:int -> number_refinement
+    | Maximum : v:int -> number_refinement
+
+type string_refinement = 
+    | MinLength : v:nat -> string_refinement
+    | MaxLength : v:nat -> string_refinement
+    | Pattern : v:string -> string_refinement
+
+type enum_refinement = 
+    | Allow : v:list string -> enum_refinement
+    | Disallow : v:list string -> enum_refinement
+
+type refinement_type =
+    | NumberRefinement : number_refinement -> refinement_type
+    | StringRefinement : string_refinement -> refinement_type
+    | EnumRefinement   : enum_refinement   -> refinement_type
+    // Some fields are restricted by (or calculated from) other fields
+    | Formula          : string            -> refinement_type
+    | And : refinement_type -> refinement_type -> refinement_type
+
+/// Primitive types
+type primitive = 
+    | Int :  primitive
+    //| Real : primitive
+    | String : primitive
+    | Boolean : primitive
+
+/// A single case discriminated union with a single field where the type name is equal to the case name
+/// NOTE: A common workaround to assign some metadata (via attributes) to a type abbreviation
+and typedef = 
+    {
+        _base : typ;
+        _attributes : value_attributes;
+    }
+
+and refinement = 
+    {
+        _base : typ;
+        _refinement : refinement_type;
+    }
+
+and enum = 
+    {
+        enum_values : list string;
+        enum_attributes : value_attributes;
+    }
+
+and array_type = 
+    | List : typ -> array_type
+    | Tuple : list typ -> array_type
+
+and array = 
+    {
+        // Refinements (like Min/Max items) included in the element_type
+        element_type : array_type;
+        _unique_items : option bool; // attributes?
+    }
+
+/// OneOf type is a discriminated union where each case has at most one field of type record
+// NOTE: An idea, a post processing step, detecting a refinement that restricts one_of to a particular case results in a flattening?
+and one_of = 
+    /// An extra enum field where its values are used to select a dependent subschema
+    | ByEnum : string -> enum -> list (string * option typ) -> one_of
+    // Add support for requiredWhen and similar
+
+and record_field = 
+    {
+        _name : string;
+        _typ : typ;
+        _isOptional : bool;
+        _attributes : value_attributes; //?
+    }
+
+and record =
+    {
+        _fields : list record_field;
+        _attributes : object_attributes;
+    }
+
+and typ = 
+    | Primitive : primitive -> typ
+    | Refinement : refinement -> typ
+    | TypeDef : typedef -> typ
+    | OneOf : one_of -> typ
+    | Array : array -> typ
+    | Enum : enum -> typ
+    | Record : record -> typ
+
+
